src/heap_lib.v
@@ -1,0 +1,120 @@
+From stdpp Require Import gmap.
+From iris.base_logic.lib Require Export own.
+From iris.proofmode Require Import tactics.
+From iris_simp_lang Require Import heap_ra.
+From iris.prelude Require Import options.
+
+(** This file is a "ghost state" library on top of heap_ra.
+
+It defines Iris propositions for owning the ghost state that will track the
+simp_lang heap and the maps-to facts that will give the right to read and write
+to it. These are built using the general Iris mechanisms for user-defined ghost
+state. Wrapping them in a library like this makes the API to the ghost state
+easier to use, since it is now stated in terms of updates in the Iris logic
+rather than theorems about the RA (so for example these theorems can be used
+directly in the IPM).
+
+*)
+
+Class gen_heapGpreS (L V : Type) (Σ : gFunctors) `{Countable L} := {
+  gen_heapGpreS_inG :> inG Σ (heap_mapR L V);
+}.
+
+Class gen_heapGS (L V : Type) (Σ : gFunctors) `{Countable L} := GenHeapGS {
+  gen_heap_inG :> gen_heapGpreS L V Σ;
+  gen_heap_name : gname;
+}.
+Global Arguments GenHeapGS L V Σ {_ _ _} _ : assert.
+Global Arguments gen_heap_name {L V Σ _ _} _ : assert.
+
+Definition gen_heapΣ (L V : Type) `{Countable L} : gFunctors := #[
+  GFunctor (heap_mapR L V)
+].
+
+Global Instance subG_gen_heapGpreS {Σ L V} `{Countable L} :
+  subG (gen_heapΣ L V) Σ → gen_heapGpreS L V Σ.
+Proof. solve_inG. Qed.
+
+Section definitions.
+  Context `{Countable L, hG : !gen_heapGS L V Σ}.
+
+  (*|
+  These two definitions are the key idea behind the state interpretation.
+  `gen_heap_interp` is the authoritative element of this RA, which will be the
+  state interpretation of `σ`, while `mapsto_def` has fragments that live outside
+  the state interpretation and are owned by threads. `l ↦ v` will be notation for
+  `mapsto`, with a full 1 fraction.
+  |*)
+
+    Definition gen_heap_interp (σ : gmap L V) : iProp Σ :=
+      own (gen_heap_name hG) (Auth (σ : gmap L V)).
+
+    Definition mapsto_def (l : L) (v: V) : iProp Σ :=
+      own (gen_heap_name hG) (Frag {[l := v]}).
+    Definition mapsto_aux : seal (@mapsto_def). Proof. by eexists. Qed.
+    Definition mapsto := mapsto_aux.(unseal).
+    Definition mapsto_eq : @mapsto = @mapsto_def := mapsto_aux.(seal_eq).
+End definitions.
+
+Notation "l ↦ v" := (mapsto l v)
+  (at level 20, format "l  ↦  v") : bi_scope.
+
+Section gen_heap.
+  Context {L V} `{Countable L, !gen_heapGS L V Σ}.
+  Implicit Types (P Q : iProp Σ).
+  Implicit Types (Φ : V → iProp Σ).
+  Implicit Types (σ : gmap L V) (l : L) (v : V).
+
+  (** General properties of mapsto *)
+  Global Instance mapsto_timeless l v : Timeless (l ↦ v).
+  Proof. rewrite mapsto_eq. apply _. Qed.
+
+  Lemma mapsto_conflict l v1 v2 : l ↦ v1 -∗ l ↦ v2 -∗ False.
+  Proof.
+    rewrite mapsto_eq. iIntros "H1 H2".
+    iDestruct (own_valid_2 with "H1 H2") as %Hdisj%heap_map_frag_frag_valid.
+    apply map_disjoint_dom in Hdisj.
+    set_solver.
+  Qed.
+
+  (** Update lemmas *)
+  Lemma gen_heap_alloc σ l v :
+    σ !! l = None →
+    gen_heap_interp σ ==∗ gen_heap_interp (<[l:=v]>σ) ∗ l ↦ v.
+  Proof.
+    iIntros (Hσl). rewrite /gen_heap_interp mapsto_eq /mapsto_def /=.
+    iIntros "Hσ".
+    iMod (own_update with "Hσ") as "[Hσ Hl]".
+    { eapply (heap_map_alloc_update _ l); done. }
+    iModIntro. iFrame.
+  Qed.
+
+  Lemma gen_heap_valid σ l v : gen_heap_interp σ -∗ l ↦ v -∗ ⌜σ !! l = Some v⌝.
+  Proof.
+    iIntros "Hσ Hl".
+    rewrite /gen_heap_interp mapsto_eq.
+    iDestruct (own_valid_2 with "Hσ Hl") as %Hsub%heap_map_auth_frag_valid.
+    iPureIntro.
+    apply map_singleton_subseteq_l in Hsub; auto.
+  Qed.
+
+  Lemma gen_heap_update σ l v1 v2 :
+    gen_heap_interp σ -∗ l ↦ v1 ==∗ gen_heap_interp (<[l:=v2]>σ) ∗ l ↦ v2.
+  Proof.
+    iIntros "Hσ Hl".
+    rewrite /gen_heap_interp mapsto_eq /mapsto_def.
+    iDestruct (own_valid_2 with "Hσ Hl") as %Hsub%heap_map_auth_frag_valid.
+    iMod (own_update_2 with "Hσ Hl") as "[Hσ Hl]".
+    { eapply heap_map_modify_update. }
+    iModIntro. iFrame.
+  Qed.
+End gen_heap.
+
+Lemma gen_heap_init `{Countable L, !gen_heapGpreS L V Σ} σ :
+  ⊢ |==> ∃ _ : gen_heapGS L V Σ, gen_heap_interp σ.
+Proof.
+  iMod (own_alloc (Auth (σ : gmap L V))) as (γ) "Hσ".
+  { exact: heap_map_auth_valid.  }
+  iExists (GenHeapGS _ _ _ γ).
+  done.
+Qed.
